simplifications

theories/StringRewriting/Reductions/HaltSBTMu_to_TSR.v
@@ -6,217 +6,22 @@ Require Undecidability.StringRewriting.SR.
 Require Import Undecidability.StringRewriting.Util.Definitions.
 Require Import Undecidability.Synthetic.Definitions.
 Require Import Undecidability.Synthetic.ReducibilityFacts.
+Require Import Undecidability.StringRewriting.Reductions.HaltSBTMu_to_SRH.
 
 Import ListNotations.
 
-Lemma nil_app_tail {X} (x : X) l : ~ [] = l ++ [x]. destruct l; cbn; firstorder congruence. Qed.
-Lemma nil_app_tail' {X} (x : X) l : ~ l ++ [x] = []. destruct l; cbn; firstorder congruence. Qed.
-
 Section FixM.
 
-    Variable M : SBTM.
+  Variable M : SBTM.  
+  Notation END := 0.
+  Notation X := 1.
+  Notation "⦇" := 2.
+  Notation "⦈" := 3.
+  Notation tt := 4.
+  Notation ff := 5.
+  Notation "!! b" := (if b then tt else ff) (at level 1).
+  Notation "! p" := (@enc_state M p) (at level 1).
 
-    Notation END := 0.
-    Notation X := 1.
-    Notation "⦇" := 2.
-    Notation "⦈" := 3.
-    Notation tt := 4.
-    Notation ff := 5.
-    Notation "!! b" := (if b then tt else ff) (at level 1).
-    Definition enc_state (q : Fin.t (S (num_states M))) := ((S ff) + proj1_sig (Fin.to_nat q)).
-    Notation "! p" := (enc_state p) (at level 1).
-
-    Fixpoint all_fins (n : nat) : list (Fin.t n) :=
-        match n with
-        | 0 => nil
-        | S n => Fin.F1 :: map Fin.FS (all_fins n)
-        end.
-
-    Lemma in_all_fins n i :
-      In i (all_fins n).
-    Proof.
-      induction i.
-      - cbn. eauto.
-      - cbn. right. eapply in_map_iff. eauto.
-    Qed.
-
-    Definition all_states {B} f : list B := flat_map f (all_fins (S (num_states M))).
-
-    Definition all_syms {B} f : list B := [f tt ; f ff].
-
-    Definition encode_sym (o : option bool) := match o with None => X | Some true => tt | Some false => ff end.
-
-    Definition encode_trans (c : option (state M * option bool * move)) (q : Fin.t (S (num_states M))) : option (nat * nat * nat * move) := 
-        option_map (fun '(s,o,m) => (!q, !s, encode_sym o, m)) c.
-
-    Definition rules q₁ : list (list nat * list nat):= 
-        match encode_trans (trans M (q₁, None)) q₁ with
-        | Some (q₁, q₂, X, Lmove) => all_syms (fun l => ([l;q₁;X], [q₂;l])) ++ [([⦇;q₁;X],[⦇;q₂;X])]
-        | Some (q₁, q₂, X, Nmove) => [([q₁;X], [q₂;X])]
-        | Some (q₁, q₂, X, Rmove) => all_syms (fun r => ([q₁;X;r], [q₂;r])) ++ [([q₁;X;⦈],[q₂;X;⦈])]
-        | Some (q₁, q₂, c, Lmove) => all_syms (fun l => ([l;q₁;X], [q₂;l;c])) ++ [([⦇;q₁;X],[⦇;q₂;X;c])]
-        | Some (q₁, q₂, c, Nmove) => [([q₁;X], [q₂;c])]
-        | Some (q₁, q₂, c, Rmove) => all_syms (fun r => ([q₁;X;r], [c;q₂;r])) ++ [([q₁;X;⦈],[c;q₂;X;⦈])]
-        | None => []
-        end ++
-        let a := tt in
-        match encode_trans (trans M (q₁, Some true)) q₁ with
-        | Some (q₁, q₂, X, Lmove) => all_syms (fun l => ([l;q₁;a], [q₂;l;a])) ++ [([⦇;q₁;a],[⦇;q₂;X;a])]
-        | Some (q₁, q₂, X, Nmove) => [([q₁;a], [q₂;a])]
-        | Some (q₁, q₂, X, Rmove) => all_syms (fun r => ([q₁;a;r], [a;q₂;r])) ++ [([q₁;a;⦈],[a;q₂;X;⦈])]
-        | Some (q₁, q₂, c, Lmove) => all_syms (fun l => ([l;q₁;a], [q₂;l;c])) ++ [([⦇;q₁;a],[⦇;q₂;X;c])]
-        | Some (q₁, q₂, c, Rmove) => all_syms (fun r => ([q₁;a;r], [c;q₂;r])) ++ [([q₁;a;⦈],[c;q₂;X;⦈])]
-        | Some (q₁, q₂, c, Nmove) => [([q₁;a], [q₂;c])]
-        | None => []
-        end ++
-        let a := ff in
-        match encode_trans (trans M (q₁, Some false)) q₁ with
-        | Some (q₁, q₂, X, Lmove) => all_syms (fun l => ([l;q₁;a], [q₂;l;a])) ++ [([⦇;q₁;a],[⦇;q₂;X;a])]
-        | Some (q₁, q₂, X, Rmove) => all_syms (fun r => ([q₁;a;r], [a;q₂;r])) ++ [([q₁;a;⦈],[a;q₂;X;⦈])]
-        | Some (q₁, q₂, X, Nmove) => [([q₁;a], [q₂;a])]
-        | Some (q₁, q₂, c, Lmove) => all_syms (fun l => ([l;q₁;a], [q₂;l;c])) ++ [([⦇;q₁;a],[⦇;q₂;X;c])]
-        | Some (q₁, q₂, c, Rmove) => all_syms (fun r => ([q₁;a;r], [c;q₂;r])) ++ [([q₁;a;⦈],[c;q₂;X;⦈])]
-        | Some (q₁, q₂, c, Nmove) => [([q₁;a], [q₂;c])]
-        | None => []
-        end.
-
-    Definition R : SR.SRS nat := all_states rules.
-
-    Lemma rules_incl q :
-      incl (rules q) R.
-    Proof.
-      unfold R, all_states.
-      intros r Hr.
-      eapply in_flat_map.
-      exists q. split; [ | assumption].
-      eapply in_all_fins.
-    Qed.
-
-    Definition enc_conf '(ls, o, rs) (q : Fin.t (S (num_states M))) : list nat :=
-      [⦇] ++ map (fun b : bool => !!b) (rev ls) ++ [!q] ++ [encode_sym o] ++ map (fun b : bool => !!b) rs ++ [⦈].
-
-    Lemma simulation q1 q2 t1 t2 :
-      eval M  q1 t1 q2 t2 -> SR.rewt R (enc_conf t1 q1) (enc_conf t2 q2).
-    Proof.
-      induction 1.
-      - econstructor.
-      - econstructor. 2:eassumption. clear - H.
-        destruct t as [[ls o] rs]. cbn in H.
-        eapply rew_subset with (2 := @rules_incl q).
-        unfold rules.
-        destruct o as [ [] | ] eqn:Eo; rewrite H; clear H.
-        1: eapply rew_subset; [ | eapply incl_appr, incl_appl, incl_refl ].
-        2: eapply rew_subset; [ | eapply incl_appr, incl_appr, incl_refl ].
-        3: eapply rew_subset; [ | eapply incl_appl, incl_refl ].
-        all:destruct w as [[] | ] eqn:Ew, m eqn:Em; cbn -[Nat.add].
-        all:try match goal with [ |- context[enc_conf match ?l with _ => _ end]] => destruct l as [ | [] ] eqn:El end; cbn -[Nat.add].
-        all: rewrite ?map_app; cbn [map app].
-        all:unfold all_syms.
-       
-        Ltac inst_left := match goal with [ |- ?L = ?R ] => 
-        match L with
-          context C [?x1 :: ?x2 :: ?x3 :: ?r] => let t := context C [@nil nat] in instantiate (2 := t)
-        | context C [?x1 :: ?x2 :: ?r] => let t := context C [@nil nat] in instantiate (2 := t)
-        end
-        end.
-        Ltac help1 := cbn -[Nat.add]; simpl_list; cbn -[Nat.add];inst_left; cbn; now simpl_list.
-        Ltac help2 := cbn -[Nat.add]; now simpl_list.
-
-        all: eapply do_rew; [ (now left + (right; now left) + (right; right; now left) + (right; right; right; now left))  | help1 | help2].
-    Qed.
-
-    Lemma enc_state_inv q t q' :
-      In (enc_state q) (enc_conf t q') -> q = q'.
-    Proof.
-      destruct t as [[ls o] rs].
-      unfold enc_conf.
-      rewrite !in_app_iff, !in_map_iff; repeat setoid_rewrite <- in_rev. cbn. firstorder try lia.
-      all: try (destruct x; lia). eapply Fin.to_nat_inj. lia. destruct o as [[]|]; cbn in *; lia.
-    Qed.
-
-    Lemma enc_conf_END t q : ~ In END (enc_conf t q).
-    Proof.
-      destruct t as [[ls o] rs].
-      unfold enc_conf.
-      rewrite !in_app_iff, !in_map_iff; repeat setoid_rewrite <- in_rev. cbn.
-      intros H. decompose [or] H; try lia; firstorder; try lia.
-      all: try (destruct x; lia). destruct o as [[]|]; cbn in *; lia.
-    Qed.
-
-    Lemma enc_conf_inv' xs q ys ls o rs q' :
-      xs ++ !q ++ ys = enc_conf (ls, o, rs) q' ->
-      xs = [⦇] ++ map (fun b : bool => !!b) (rev ls) /\
-      q = q' /\
-      ys = encode_sym o :: map (fun b : bool => !!b) rs ++ [⦈].
-    Proof.
-      intros. pose proof (H' := H). cbn - [Nat.add] in H.
-      destruct xs; cbn -[Nat.add] in H; inversion H; subst n; clear H.
-
-      eapply list_prefix_inv' in H2 as (H1 & -> & H3).
-      - subst. repeat split. eapply Fin.to_nat_inj. unfold "!" in H1. lia.
-      - clear H'. induction xs in ls, H2 |- *.
-        + firstorder.
-        + cbn -[Nat.add]. destruct ls as [ | ? ? _] using rev_ind.
-          * cbn -[Nat.add] in H2. inversion H2. subst. destruct xs; inversion H1; subst.
-            destruct o as [ [] | ]; cbn in H0; lia.
-            assert (In (!q) (map (fun b : bool => !! b) rs ++ [⦈])). rewrite <- H3. rewrite in_app_iff. cbn[In]. solve [eauto].
-            eapply in_app_iff in H as [ (? & ? & ?) % in_map_iff | [ | []]]; try destruct x; cbn in H; lia.
-          * rewrite rev_app_distr in H2. cbn -[Nat.add] in H2. inversion H2; subst.
-            intros [ | ].
-            -- destruct x; cbn in *; lia.
-            -- eapply IHxs. 2:eauto. rewrite H1. reflexivity.
-      - intros (? & ? & ?) % in_map_iff. destruct x; cbn in *; lia.
-    Qed.
-
-    Lemma enc_conf_inv xs q c ys ls o rs q' :
-      xs ++ !q ++ [c] ++ ys = enc_conf (ls, o, rs) q' ->
-      xs = [⦇] ++ map (fun b : bool => !!b) (rev ls) /\
-      q = q' /\
-      c = encode_sym o /\
-      ys = map (fun b : bool => !!b) rs ++ [⦈].
-    Proof.
-      intros. eapply enc_conf_inv' in H as (-> & -> & [= -> ->]). eauto.
-    Qed.
-
-    Definition swap {X Y} : X * Y -> Y * X := fun '(x,y) => (y,x).
-
-    Lemma rev_sim t q z : 
-      SR.rew R (enc_conf t q) z -> exists q' w m, trans M (q, curr t) = Some (q', w, m) /\ z = enc_conf (mv m (wr w t)) q'.
-    Proof.
-      intros H. inversion H as [x y u v Hin HL HR]; subst z.
-      destruct t as [[ls o] rs]. 
-      eapply in_flat_map in Hin as (q_ & _ & Hq2).
-      unfold rules in Hq2.
-      rewrite ! in_app_iff in Hq2.
-      destruct Hq2 as [ Hq2 | [Hq2 | Hq2]].
-      all: destruct (trans M (q_, _)) as [ [[q' w] m] | ] eqn:Etrans; try destruct m eqn:Em;
-          try destruct w as [[] | ] eqn:Ew; cbn -[Nat.add] in Hq2; (exists q', w, m || exfalso); rewrite ?Em, ?Ew.
-      all: repeat match type of Hq2 with _ \/ _ => destruct Hq2 as [Hq2 | Hq2] end; inversion Hq2; subst u v; clear Hq2; cbn -[Nat.add].
-
-      cbn [app] in HL.
-      all:
-          cbn [app] in HL;
-          match type of HL with
-          | ?L = ?R => match L with context C [! ?q :: ?c :: ?rs] => let ls := context C [@nil nat] in 
-           replace L with (ls ++ !q ++ [c] ++ rs) in HL; [ | cbn; now simpl_list]
-          end
-          end.
-
-    all:
-        match type of HL with _ = enc_conf (?ls,?o,?rs) ?q =>
-        let H1 := fresh "H" in let H2 := fresh "H" in let H3 := fresh "H" in let H4 := fresh "H" in let HH := fresh "H" in
-        eapply enc_conf_inv in HL as (H1 & -> & H3 & H4); try rewrite H4 in *; destruct o as [ [] | ]; inversion H3; clear H3; cbn in H1;
-        rewrite ?app_nil_r in H1; subst;
-        split ; try eassumption; try reflexivity;
-        (let x := match type of H1 with ?x ++ _ = _ => x end in
-        destruct x; try (now inversion H1); cbn in H1; eapply cons_inj in H1 as [HH H1]; try rewrite HH in *; clear HH;
-        now destruct ls as [ | []]; cbn in H1; 
-        [ reflexivity || destruct x; now inversion H1 | try rewrite map_app in H1; cbn in H1; (eapply app_inj_tail in H1 as [-> [=]] + (try eapply nil_app_tail in H1 as []) + (try eapply nil_app_tail' in H1 as []) ).. ])
-        + (destruct rs as [ | [] rs]; cbn in H4; eapply cons_inj in H4 as [ [=] H4]; rewrite ?H4 in *; clear H4;
-           now cbn; simpl_list)
-         end.
-  Qed.
-  
   Lemma help_exists1 (P : state M -> tape -> option bool -> move -> Prop) :
     (exists c q w m ls rs, P q (ls, c, rs) w m) ->  (exists q t w m, P q t w m).
   Proof.
@@ -230,7 +35,7 @@ Section FixM.
   Qed.
 
   Lemma rev_sim_swap t q z : 
-  SR.rew (map swap R) (enc_conf t q) z -> exists q' t' w m, trans M (q', curr t') = Some (q, w, m) /\ t = mv m (wr w t') /\ z = enc_conf t' q'.
+    SR.rew (map SR.swap (R M)) (enc_conf t q) z -> exists q' t' w m, trans M (q', curr t') = Some (q, w, m) /\ t = mv m (wr w t') /\ z = enc_conf t' q'.
   Proof.
     intros H. inversion H as [x y v u Hin HL HR]; subst z.
     eapply in_map_iff in Hin as ([? ?] & [= -> ->] & Hin).
@@ -357,9 +162,18 @@ Section FixM.
       eapply app_inj_tail in H4 as [H4 [=]].
     1,2: destruct rs as [ | []]; inversion H2; eauto.
   Qed.
-
+  
+  Lemma enc_conf_END t q : ~ In END (@enc_conf M t q).
+  Proof.
+    destruct t as [[ls o] rs].
+    unfold enc_conf.
+    rewrite !in_app_iff, !in_map_iff; repeat setoid_rewrite <- in_rev. cbn.
+    intros H. decompose [or] H; try lia; firstorder; try lia.
+    all: try (destruct x; lia). destruct o as [[]|]; cbn in *; lia.
+  Qed.
+  
   Lemma rev_sim_Del_swap t q z : 
-    SR.rew (map swap Del) (enc_conf t q) z -> q = q_halt /\ exists t',  z = enc_conf t' q_halt.
+    SR.rew (map SR.swap Del) (enc_conf t q) z -> q = q_halt /\ exists t',  z = enc_conf t' q_halt.
   Proof.
     intros H. inversion H as [x y v u Hin HL HR]; subst z.
     cbn -[Nat.add] in Hin.
@@ -388,33 +202,7 @@ Section FixM.
     all: edestruct enc_conf_END; rewrite <- HL; eauto.
   Qed.
 
-  Lemma rev_sim_END z :
-    ~ SR.rew (R ++ map swap R) [END] z.
-  Proof.
-    intros H. inversion H as [x y v u Hin HL HR]; subst z.
-    eapply in_app_iff in Hin as [Hin | Hin].
-    2: eapply in_map_iff in Hin as ([] & [= -> ->] & Hin).
-    all: eapply in_flat_map in Hin as (q_ & _ & Hq2).
-    all: unfold rules in Hq2.
-    all: rewrite ! in_app_iff in Hq2.
-    all: destruct Hq2 as [Hq2 | [Hq2 | Hq2]].
-      all: destruct (trans M (q_, _)) as [ [[q' w] m] | ] eqn:Etrans; try destruct m eqn:Em;
-       try destruct w as [[] | ] eqn:Ew; cbn -[Nat.add] in Hq2; decompose [or] Hq2.
-      all: try specialize H0 as [= <- <-]. all: try specialize H1 as [= <- <-].
-      all: try now destruct x as [ | ? []]; inversion HL.
-  Qed.
-
 End FixM.
-
-Lemma rew_app_inv (R1 R2 : SR.SRS nat) x y :
-  SR.rew (R1 ++ R2) x y <-> SR.rew R1 x y \/ SR.rew R2 x y.
-Proof.
-  split.
-  - inversion 1 as [x0 y0 u v H0]; subst; eapply in_app_iff in H0 as [H0 | H0].
-    + left. econstructor. eauto.
-    + right. econstructor. eauto.
-  - intros [H | H]; eapply rew_subset; eauto.
-Qed.
 
 Lemma backwards M t q1 q:
   (forall c, trans M (q,c) = None /\ (forall q', trans M (q', c) = None -> q' = q)) ->
@@ -449,4 +237,4 @@ Proof.
       + eapply rewt_subset. eapply simulation. eassumption. eauto.
       + eapply rewt_subset. eapply sim_Del. eauto.
     - cbn -[Del R Nat.add]. intros H1. now eapply (backwards Hq).
-Qed.
+Qed. 
